stanfrontend/Sbackendproof.v
@@ -29,8 +29,8 @@ Inductive match_states: CStan.state -> Clight.state -> Prop :=
       match_states (CStan.State f s k e le m t)
                    (Clight.State tf ts tk e le m)
   | match_call_state:
-      forall fd vargs k m t tfd tk i
-      (TRFD: transf_fundef i fd = OK tfd)
+      forall fd vargs k m t tfd tk
+      (TRFD: transf_fundef fd = OK tfd)
       (MCONT: match_cont k tk),
       match_states (CStan.Callstate fd vargs k m t)
                    (Clight.Callstate tfd vargs tk m)
@@ -40,423 +40,204 @@ Inductive match_states: CStan.state -> Clight.state -> Prop :=
       match_states (CStan.Returnstate v k m t)
                    (Clight.Returnstate v tk m).
 
-(** ** Top-level translation *)
 
-(** The "top-level" translation is equivalent to [tr_expr] above
-  for source terms.  It brings additional flexibility in the matching
-  between Csyntax values and Cminor expressions: in the case of
-  [tr_expr], the Cminor expression must not depend on memory,
-  while in the case of [tr_top] it can depend on the current memory
-  state. *)
-
-Section TR_TOP.
-
-Variable e: CStan.env.
-Variable le: CStan.temp_env.
-Variable m: mem.
-
-Variable ta: Floats.float. (* target *)
-
-(* Inductive tr_expr: temp_env -> CStan.expr -> expr -> list AST.ident -> Prop := *)
-(*   | tr_var: forall le id ty tmp, *)
-(*       tr_expr le (CStan.Evar id ty) (Evar id ty) tmp *)
-(*   | tr_deref: forall le e1 ty sl1 a1 tmp, *)
-(*       tr_expr le e1 sl1 a1 tmp -> *)
-(*       tr_expr le (CStan.Ederef e1 ty) *)
-(*               (sl1 ++ final (Ederef' a1 ty)) (Ederef' a1 ty) tmp *)
-(*   | tr_field: forall le dst e1 f ty sl1 a1 tmp, *)
-(*       tr_expr le e1 sl1 a1 tmp -> *)
-(*       tr_expr le (CStan.Efield e1 f ty) *)
-(*               (sl1 ++ final dst (Efield a1 f ty)) (Efield a1 f ty) tmp *)
-(* (*   | tr_val_effect: forall le v ty any tmp, *) *)
-(* (*       tr_expr le For_effects (CStan.Eval v ty) nil any tmp *) *)
-(* (*   | tr_val_value: forall le v ty a tmp, *) *)
-(* (*       typeof a = ty -> *) *)
-(* (*       (forall tge e le' m, *) *)
-(* (*          (forall id, In id tmp -> le'!id = le!id) -> *) *)
-(* (*          eval_expr tge e le' m a v) -> *) *)
-(* (*       tr_expr le For_val (CStan.Eval v ty) *) *)
-(* (*                            nil a tmp *) *)
-(* (*   | tr_val_set: forall le sd v ty a any tmp, *) *)
-(* (*       typeof a = ty -> *) *)
-(* (*       (forall tge e le' m, *) *)
-(* (*          (forall id, In id tmp -> le'!id = le!id) -> *) *)
-(* (*          eval_expr tge e le' m a v) -> *) *)
-(* (*       tr_expr le (For_set sd) (CStan.Eval v ty) *) *)
-(* (*                    (do_set sd a) any tmp *) *)
-(* (*   | tr_sizeof: forall le dst ty' ty tmp, *) *)
-(* (*       tr_expr le dst (CStan.Esizeof ty' ty) *) *)
-(* (*                    (final dst (Esizeof ty' ty)) *) *)
-(* (*                    (Esizeof ty' ty) tmp *) *)
-(* (*   | tr_alignof: forall le dst ty' ty tmp, *) *)
-(* (*       tr_expr le dst (CStan.Ealignof ty' ty) *) *)
-(* (*                    (final dst (Ealignof ty' ty)) *) *)
-(* (*                    (Ealignof ty' ty) tmp *) *)
-(* (*   | tr_valof: forall le dst e1 ty tmp sl1 a1 tmp1 sl2 a2 tmp2, *) *)
-(* (*       tr_expr le For_val e1 sl1 a1 tmp1 -> *) *)
-(* (*       tr_rvalof (CStan.typeof e1) a1 sl2 a2 tmp2 -> *) *)
-(* (*       list_disjoint tmp1 tmp2 -> incl tmp1 tmp -> incl tmp2 tmp -> *) *)
-(* (*       tr_expr le dst (CStan.Evalof e1 ty) *) *)
-(* (*                     (sl1 ++ sl2 ++ final dst a2) *) *)
-(* (*                     a2 tmp *) *)
-(* (*   | tr_addrof: forall le dst e1 ty tmp sl1 a1, *) *)
-(* (*       tr_expr le For_val e1 sl1 a1 tmp -> *) *)
-(* (*       tr_expr le dst (Csyntax.Eaddrof e1 ty) *) *)
-(* (*                    (sl1 ++ final dst (Eaddrof' a1 ty)) *) *)
-(* (*                    (Eaddrof' a1 ty) tmp *) *)
-(* (*   | tr_unop: forall le dst op e1 ty tmp sl1 a1, *) *)
-(* (*       tr_expr le For_val e1 sl1 a1 tmp -> *) *)
-(* (*       tr_expr le dst (Csyntax.Eunop op e1 ty) *) *)
-(* (*                    (sl1 ++ final dst (Eunop op a1 ty)) *) *)
-(* (*                    (Eunop op a1 ty) tmp *) *)
-(* (*   | tr_binop: forall le dst op e1 e2 ty sl1 a1 tmp1 sl2 a2 tmp2 tmp, *) *)
-(* (*       tr_expr le For_val e1 sl1 a1 tmp1 -> *) *)
-(* (*       tr_expr le For_val e2 sl2 a2 tmp2 -> *) *)
-(* (*       list_disjoint tmp1 tmp2 -> incl tmp1 tmp -> incl tmp2 tmp -> *) *)
-(* (*       tr_expr le dst (Csyntax.Ebinop op e1 e2 ty) *) *)
-(* (*                    (sl1 ++ sl2 ++ final dst (Ebinop op a1 a2 ty)) *) *)
-(* (*                    (Ebinop op a1 a2 ty) tmp *) *)
-(* (*   | tr_cast_effects: forall le e1 ty sl1 a1 any tmp, *) *)
-(* (*       tr_expr le For_effects e1 sl1 a1 tmp -> *) *)
-(* (*       tr_expr le For_effects (Csyntax.Ecast e1 ty) *) *)
-(* (*                    sl1 *) *)
-(* (*                    any tmp *) *)
-(* (*   | tr_cast_val: forall le dst e1 ty sl1 a1 tmp, *) *)
-(* (*       tr_expr le For_val e1 sl1 a1 tmp -> *) *)
-(* (*       tr_expr le dst (Csyntax.Ecast e1 ty) *) *)
-(* (*                    (sl1 ++ final dst (Ecast a1 ty)) *) *)
-(* (*                    (Ecast a1 ty) tmp *) *)
-(* (*   | tr_seqand_val: forall le e1 e2 ty sl1 a1 tmp1 t sl2 a2 tmp2 tmp, *) *)
-(* (*       tr_expr le For_val e1 sl1 a1 tmp1 -> *) *)
-(* (*       tr_expr le (For_set (sd_seqbool_val t ty)) e2 sl2 a2 tmp2 -> *) *)
-(* (*       list_disjoint tmp1 tmp2 -> *) *)
-(* (*       incl tmp1 tmp -> incl tmp2 tmp -> In t tmp -> *) *)
-(* (*       tr_expr le For_val (Csyntax.Eseqand e1 e2 ty) *) *)
-(* (*                     (sl1 ++ makeif a1 (makeseq sl2) *) *)
-(* (*                                       (Sset t (Econst_int Int.zero ty)) :: nil) *) *)
-(* (*                     (Etempvar t ty) tmp *) *)
-(* (*   | tr_seqand_effects: forall le e1 e2 ty sl1 a1 tmp1 sl2 a2 tmp2 any tmp, *) *)
-(* (*       tr_expr le For_val e1 sl1 a1 tmp1 -> *) *)
-(* (*       tr_expr le For_effects e2 sl2 a2 tmp2 -> *) *)
-(* (*       list_disjoint tmp1 tmp2 -> *) *)
-(* (*       incl tmp1 tmp -> incl tmp2 tmp -> *) *)
-(* (*       tr_expr le For_effects (Csyntax.Eseqand e1 e2 ty) *) *)
-(* (*                     (sl1 ++ makeif a1 (makeseq sl2) Sskip :: nil) *) *)
-(* (*                     any tmp *) *)
-(* (*   | tr_seqand_set: forall le sd e1 e2 ty sl1 a1 tmp1 sl2 a2 tmp2 any tmp, *) *)
-(* (*       tr_expr le For_val e1 sl1 a1 tmp1 -> *) *)
-(* (*       tr_expr le (For_set (sd_seqbool_set ty sd)) e2 sl2 a2 tmp2 -> *) *)
-(* (*       list_disjoint tmp1 tmp2 -> *) *)
-(* (*       incl tmp1 tmp -> incl tmp2 tmp -> In (sd_temp sd) tmp -> *) *)
-(* (*       tr_expr le (For_set sd) (Csyntax.Eseqand e1 e2 ty) *) *)
-(* (*                     (sl1 ++ makeif a1 (makeseq sl2) *) *)
-(* (*                                       (makeseq (do_set sd (Econst_int Int.zero ty))) :: nil) *) *)
-(* (*                     any tmp *) *)
-(* (*   | tr_seqor_val: forall le e1 e2 ty sl1 a1 tmp1 t sl2 a2 tmp2 tmp, *) *)
-(* (*       tr_expr le For_val e1 sl1 a1 tmp1 -> *) *)
-(* (*       tr_expr le (For_set (sd_seqbool_val t ty)) e2 sl2 a2 tmp2 -> *) *)
-(* (*       list_disjoint tmp1 tmp2 -> *) *)
-(* (*       incl tmp1 tmp -> incl tmp2 tmp -> In t tmp -> *) *)
-(* (*       tr_expr le For_val (Csyntax.Eseqor e1 e2 ty) *) *)
-(* (*                     (sl1 ++ makeif a1 (Sset t (Econst_int Int.one ty)) *) *)
-(* (*                                       (makeseq sl2) :: nil) *) *)
-(* (*                     (Etempvar t ty) tmp *) *)
-(* (*   | tr_seqor_effects: forall le e1 e2 ty sl1 a1 tmp1 sl2 a2 tmp2 any tmp, *) *)
-(* (*       tr_expr le For_val e1 sl1 a1 tmp1 -> *) *)
-(* (*       tr_expr le For_effects e2 sl2 a2 tmp2 -> *) *)
-(* (*       list_disjoint tmp1 tmp2 -> *) *)
-(* (*       incl tmp1 tmp -> incl tmp2 tmp -> *) *)
-(* (*       tr_expr le For_effects (Csyntax.Eseqor e1 e2 ty) *) *)
-(* (*                     (sl1 ++ makeif a1 Sskip (makeseq sl2) :: nil) *) *)
-(* (*                     any tmp *) *)
-(* (*   | tr_seqor_set: forall le sd e1 e2 ty sl1 a1 tmp1 sl2 a2 tmp2 any tmp, *) *)
-(* (*       tr_expr le For_val e1 sl1 a1 tmp1 -> *) *)
-(* (*       tr_expr le (For_set (sd_seqbool_set ty sd)) e2 sl2 a2 tmp2 -> *) *)
-(* (*       list_disjoint tmp1 tmp2 -> *) *)
-(* (*       incl tmp1 tmp -> incl tmp2 tmp -> In (sd_temp sd) tmp -> *) *)
-(* (*       tr_expr le (For_set sd) (Csyntax.Eseqor e1 e2 ty) *) *)
-(* (*                     (sl1 ++ makeif a1 (makeseq (do_set sd (Econst_int Int.one ty))) *) *)
-(* (*                                       (makeseq sl2) :: nil) *) *)
-(* (*                     any tmp *) *)
-(* (*   | tr_condition_val: forall le e1 e2 e3 ty sl1 a1 tmp1 sl2 a2 tmp2 sl3 a3 tmp3 t tmp, *) *)
-(* (*       tr_expr le For_val e1 sl1 a1 tmp1 -> *) *)
-(* (*       tr_expr le (For_set (SDbase ty ty t)) e2 sl2 a2 tmp2 -> *) *)
-(* (*       tr_expr le (For_set (SDbase ty ty t)) e3 sl3 a3 tmp3 -> *) *)
-(* (*       list_disjoint tmp1 tmp2 -> *) *)
-(* (*       list_disjoint tmp1 tmp3 -> *) *)
-(* (*       incl tmp1 tmp -> incl tmp2 tmp ->  incl tmp3 tmp -> In t tmp -> *) *)
-(* (*       tr_expr le For_val (Csyntax.Econdition e1 e2 e3 ty) *) *)
-(* (*                       (sl1 ++ makeif a1 (makeseq sl2) (makeseq sl3) :: nil) *) *)
-(* (*                       (Etempvar t ty) tmp *) *)
-(* (*   | tr_condition_effects: forall le e1 e2 e3 ty sl1 a1 tmp1 sl2 a2 tmp2 sl3 a3 tmp3 any tmp, *) *)
-(* (*       tr_expr le For_val e1 sl1 a1 tmp1 -> *) *)
-(* (*       tr_expr le For_effects e2 sl2 a2 tmp2 -> *) *)
-(* (*       tr_expr le For_effects e3 sl3 a3 tmp3 -> *) *)
-(* (*       list_disjoint tmp1 tmp2 -> *) *)
-(* (*       list_disjoint tmp1 tmp3 -> *) *)
-(* (*       incl tmp1 tmp -> incl tmp2 tmp -> incl tmp3 tmp -> *) *)
-(* (*       tr_expr le For_effects (Csyntax.Econdition e1 e2 e3 ty) *) *)
-(* (*                        (sl1 ++ makeif a1 (makeseq sl2) (makeseq sl3) :: nil) *) *)
-(* (*                        any tmp *) *)
-(* (*   | tr_condition_set: forall le sd t e1 e2 e3 ty sl1 a1 tmp1 sl2 a2 tmp2 sl3 a3 tmp3 any tmp, *) *)
-(* (*       tr_expr le For_val e1 sl1 a1 tmp1 -> *) *)
-(* (*       tr_expr le (For_set (SDcons ty ty t sd)) e2 sl2 a2 tmp2 -> *) *)
-(* (*       tr_expr le (For_set (SDcons ty ty t sd)) e3 sl3 a3 tmp3 -> *) *)
-(* (*       list_disjoint tmp1 tmp2 -> *) *)
-(* (*       list_disjoint tmp1 tmp3 -> *) *)
-(* (*       incl tmp1 tmp -> incl tmp2 tmp -> incl tmp3 tmp -> In t tmp -> *) *)
-(* (*       tr_expr le (For_set sd) (Csyntax.Econdition e1 e2 e3 ty) *) *)
-(* (*                        (sl1 ++ makeif a1 (makeseq sl2) (makeseq sl3) :: nil) *) *)
-(* (*                        any tmp *) *)
-(* (*   | tr_assign_effects: forall le e1 e2 ty sl1 a1 tmp1 sl2 a2 tmp2 any tmp, *) *)
-(* (*       tr_expr le For_val e1 sl1 a1 tmp1 -> *) *)
-(* (*       tr_expr le For_val e2 sl2 a2 tmp2 -> *) *)
-(* (*       list_disjoint tmp1 tmp2 -> *) *)
-(* (*       incl tmp1 tmp -> incl tmp2 tmp -> *) *)
-(* (*       tr_expr le For_effects (Csyntax.Eassign e1 e2 ty) *) *)
-(* (*                       (sl1 ++ sl2 ++ make_assign a1 a2 :: nil) *) *)
-(* (*                       any tmp *) *)
-(* (*   | tr_assign_val: forall le dst e1 e2 ty sl1 a1 tmp1 sl2 a2 tmp2 t tmp ty1 ty2, *) *)
-(* (*       tr_expr le For_val e1 sl1 a1 tmp1 -> *) *)
-(* (*       tr_expr le For_val e2 sl2 a2 tmp2 -> *) *)
-(* (*       incl tmp1 tmp -> incl tmp2 tmp -> *) *)
-(* (*       list_disjoint tmp1 tmp2 -> *) *)
-(* (*       In t tmp -> ~In t tmp1 -> ~In t tmp2 -> *) *)
-(* (*       ty1 = Csyntax.typeof e1 -> *) *)
-(* (*       ty2 = Csyntax.typeof e2 -> *) *)
-(* (*       tr_expr le dst (Csyntax.Eassign e1 e2 ty) *) *)
-(* (*                    (sl1 ++ sl2 ++ *) *)
-(* (*                     Sset t (Ecast a2 ty1) :: *) *)
-(* (*                     make_assign a1 (Etempvar t ty1) :: *) *)
-(* (*                     final dst (Etempvar t ty1)) *) *)
-(* (*                    (Etempvar t ty1) tmp *) *)
-(* (*   | tr_assignop_effects: forall le op e1 e2 tyres ty ty1 sl1 a1 tmp1 sl2 a2 tmp2 sl3 a3 tmp3 any tmp, *) *)
-(* (*       tr_expr le For_val e1 sl1 a1 tmp1 -> *) *)
-(* (*       tr_expr le For_val e2 sl2 a2 tmp2 -> *) *)
-(* (*       ty1 = Csyntax.typeof e1 -> *) *)
-(* (*       tr_rvalof ty1 a1 sl3 a3 tmp3 -> *) *)
-(* (*       list_disjoint tmp1 tmp2 -> list_disjoint tmp1 tmp3 -> list_disjoint tmp2 tmp3 -> *) *)
-(* (*       incl tmp1 tmp -> incl tmp2 tmp -> incl tmp3 tmp -> *) *)
-(* (*       tr_expr le For_effects (Csyntax.Eassignop op e1 e2 tyres ty) *) *)
-(* (*                       (sl1 ++ sl2 ++ sl3 ++ make_assign a1 (Ebinop op a3 a2 tyres) :: nil) *) *)
-(* (*                       any tmp *) *)
-(* (*   | tr_assignop_val: forall le dst op e1 e2 tyres ty sl1 a1 tmp1 sl2 a2 tmp2 sl3 a3 tmp3 t tmp ty1, *) *)
-(* (*       tr_expr le For_val e1 sl1 a1 tmp1 -> *) *)
-(* (*       tr_expr le For_val e2 sl2 a2 tmp2 -> *) *)
-(* (*       tr_rvalof ty1 a1 sl3 a3 tmp3 -> *) *)
-(* (*       list_disjoint tmp1 tmp2 -> list_disjoint tmp1 tmp3 -> list_disjoint tmp2 tmp3 -> *) *)
-(* (*       incl tmp1 tmp -> incl tmp2 tmp -> incl tmp3 tmp -> *) *)
-(* (*       In t tmp -> ~In t tmp1 -> ~In t tmp2 -> ~In t tmp3 -> *) *)
-(* (*       ty1 = Csyntax.typeof e1 -> *) *)
-(* (*       tr_expr le dst (Csyntax.Eassignop op e1 e2 tyres ty) *) *)
-(* (*                    (sl1 ++ sl2 ++ sl3 ++ *) *)
-(* (*                     Sset t (Ecast (Ebinop op a3 a2 tyres) ty1) :: *) *)
-(* (*                     make_assign a1 (Etempvar t ty1) :: *) *)
-(* (*                     final dst (Etempvar t ty1)) *) *)
-(* (*                    (Etempvar t ty1) tmp *) *)
-(* (*   | tr_postincr_effects: forall le id e1 ty ty1 sl1 a1 tmp1 sl2 a2 tmp2 any tmp, *) *)
-(* (*       tr_expr le For_val e1 sl1 a1 tmp1 -> *) *)
-(* (*       tr_rvalof ty1 a1 sl2 a2 tmp2 -> *) *)
-(* (*       ty1 = Csyntax.typeof e1 -> *) *)
-(* (*       incl tmp1 tmp -> incl tmp2 tmp -> *) *)
-(* (*       list_disjoint tmp1 tmp2 -> *) *)
-(* (*       tr_expr le For_effects (Csyntax.Epostincr id e1 ty) *) *)
-(* (*                       (sl1 ++ sl2 ++ make_assign a1 (transl_incrdecr id a2 ty1) :: nil) *) *)
-(* (*                       any tmp *) *)
-(* (*   | tr_postincr_val: forall le dst id e1 ty sl1 a1 tmp1 t ty1 tmp, *) *)
-(* (*       tr_expr le For_val e1 sl1 a1 tmp1 -> *) *)
-(* (*       incl tmp1 tmp -> In t tmp -> ~In t tmp1 -> *) *)
-(* (*       ty1 = Csyntax.typeof e1 -> *) *)
-(* (*       tr_expr le dst (Csyntax.Epostincr id e1 ty) *) *)
-(* (*                    (sl1 ++ make_set t a1 :: *) *)
-(* (*                     make_assign a1 (transl_incrdecr id (Etempvar t ty1) ty1) :: *) *)
-(* (*                     final dst (Etempvar t ty1)) *) *)
-(* (*                    (Etempvar t ty1) tmp *) *)
-(* (*   | tr_comma: forall le dst e1 e2 ty sl1 a1 tmp1 sl2 a2 tmp2 tmp, *) *)
-(* (*       tr_expr le For_effects e1 sl1 a1 tmp1 -> *) *)
-(* (*       tr_expr le dst e2 sl2 a2 tmp2 -> *) *)
-(* (*       list_disjoint tmp1 tmp2 -> *) *)
-(* (*       incl tmp1 tmp -> incl tmp2 tmp -> *) *)
-(* (*       tr_expr le dst (Csyntax.Ecomma e1 e2 ty) (sl1 ++ sl2) a2 tmp *) *)
-(* (*   | tr_call_effects: forall le e1 el2 ty sl1 a1 tmp1 sl2 al2 tmp2 any tmp, *) *)
-(* (*       tr_expr le For_val e1 sl1 a1 tmp1 -> *) *)
-(* (*       tr_exprlist le el2 sl2 al2 tmp2 -> *) *)
-(* (*       list_disjoint tmp1 tmp2 -> *) *)
-(* (*       incl tmp1 tmp -> incl tmp2 tmp -> *) *)
-(* (*       tr_expr le For_effects (Csyntax.Ecall e1 el2 ty) *) *)
-(* (*                    (sl1 ++ sl2 ++ Scall None a1 al2 :: nil) *) *)
-(* (*                    any tmp *) *)
-(* (*   | tr_call_val: forall le dst e1 el2 ty sl1 a1 tmp1 sl2 al2 tmp2 t tmp, *) *)
-(* (*       dst <> For_effects -> *) *)
-(* (*       tr_expr le For_val e1 sl1 a1 tmp1 -> *) *)
-(* (*       tr_exprlist le el2 sl2 al2 tmp2 -> *) *)
-(* (*       list_disjoint tmp1 tmp2 -> In t tmp -> *) *)
-(* (*       incl tmp1 tmp -> incl tmp2 tmp -> *) *)
-(* (*       tr_expr le dst (Csyntax.Ecall e1 el2 ty) *) *)
-(* (*                    (sl1 ++ sl2 ++ Scall (Some t) a1 al2 :: final dst (Etempvar t ty)) *) *)
-(* (*                    (Etempvar t ty) tmp *) *)
-(* (*   | tr_builtin_effects: forall le ef tyargs el ty sl al tmp1 any tmp, *) *)
-(* (*       tr_exprlist le el sl al tmp1 -> *) *)
-(* (*       incl tmp1 tmp -> *) *)
-(* (*       tr_expr le For_effects (Csyntax.Ebuiltin ef tyargs el ty) *) *)
-(* (*                    (sl ++ Sbuiltin None ef tyargs al :: nil) *) *)
-(* (*                    any tmp *) *)
-(* (*   | tr_builtin_val: forall le dst ef tyargs el ty sl al tmp1 t tmp, *) *)
-(* (*       dst <> For_effects -> *) *)
-(* (*       tr_exprlist le el sl al tmp1 -> *) *)
-(* (*       In t tmp -> incl tmp1 tmp -> *) *)
-(* (*       tr_expr le dst (Csyntax.Ebuiltin ef tyargs el ty) *) *)
-(* (*                    (sl ++ Sbuiltin (Some t) ef tyargs al :: final dst (Etempvar t ty)) *) *)
-(* (*                    (Etempvar t ty) tmp *) *)
-(* (*   | tr_paren_val: forall le e1 tycast ty sl1 a1 t tmp, *) *)
-(* (*       tr_expr le (For_set (SDbase tycast ty t)) e1 sl1 a1 tmp -> *) *)
-(* (*       In t tmp -> *) *)
-(* (*       tr_expr le For_val (Csyntax.Eparen e1 tycast ty) *) *)
-(* (*                        sl1 *) *)
-(* (*                        (Etempvar t ty) tmp *) *)
-(* (*   | tr_paren_effects: forall le e1 tycast ty sl1 a1 tmp any, *) *)
-(* (*       tr_expr le For_effects e1 sl1 a1 tmp -> *) *)
-(* (*       tr_expr le For_effects (Csyntax.Eparen e1 tycast ty) sl1 any tmp *) *)
-(* (*   | tr_paren_set: forall le t sd e1 tycast ty sl1 a1 tmp any, *) *)
-(* (*       tr_expr le (For_set (SDcons tycast ty t sd)) e1 sl1 a1 tmp -> *) *)
-(* (*       In t tmp -> *) *)
-(* (*       tr_expr le (For_set sd) (Csyntax.Eparen e1 tycast ty) sl1 any tmp *) *)
-
-(* (* with tr_exprlist: temp_env -> Csyntax.exprlist -> list statement -> list expr -> list ident -> Prop := *) *)
-(* (*   | tr_nil: forall le tmp, *) *)
-(* (*       tr_exprlist le Csyntax.Enil nil nil tmp *) *)
-(* (*   | tr_cons: forall le e1 el2 sl1 a1 tmp1 sl2 al2 tmp2 tmp, *) *)
-(* (*       tr_expr le For_val e1 sl1 a1 tmp1 -> *) *)
-(* (*       tr_exprlist le el2 sl2 al2 tmp2 -> *) *)
-(* (*       list_disjoint tmp1 tmp2 -> *) *)
-(* (*       incl tmp1 tmp -> incl tmp2 tmp -> *) *)
-(* (*       tr_exprlist le (Csyntax.Econs e1 el2) (sl1 ++ sl2) (a1 :: al2) tmp *) *)
-(*   . *)
-
-
-Inductive tr_top: CStan.expr -> list statement -> expr -> list AST.ident -> Prop :=
-  | tr_top_val_int: forall i ty a tmp,
-      typeof a = ty -> eval_expr tge e le m a (Values.Vint i) ->
-      tr_top (CStan.Econst_int i ty) nil a tmp
-   | tr_top_val_long: forall i ty a tmp,
-      typeof a = ty -> eval_expr tge e le m a (Values.Vlong i) ->
-      tr_top (CStan.Econst_int (Int.repr (Int64.unsigned i)) ty) nil a tmp
-  (* ... more? ... *)
-
-  | tr_top_val_float: forall f ty a tmp,
-      typeof a = ty -> eval_expr tge e le m a (Values.Vfloat f) ->
-      tr_top (CStan.Econst_float f ty) nil a tmp
-
-  (* missing: *)
-  (* | Vundef: val *)
-  (* | Vsingle: float32 -> val *)
-  (* | Vptr: block -> ptrofs -> val. *)
-
-  (* also the recursive call: *)
-  (* | tr_top_base: forall r sl a tmp, *)
-  (*     tr_expr le dst r sl a tmp -> *)
-  (*     tr_top r sl a tmp. *)
-  .
-
-End TR_TOP.
-
-
-Lemma tr_expression: CStan.expr -> Clight.statement -> Clight.expr -> Prop.
-Admitted.
-
-Lemma tr_stmt: CStan.statement -> statement -> Prop.
-Admitted.
-  (* | tr_skip: *)
-  (*     tr_stmt CStan.Sskip Sskip *)
-  (* | tr_seq: forall s1 s2 ts1 ts2, *)
-  (*     tr_stmt s1 ts1 -> tr_stmt s2 ts2 -> *)
-  (*     tr_stmt (CStan.Ssequence s1 s2) (Ssequence ts1 ts2) *)
-  (* | tr_ifthenelse_empty: forall r s' a, *)
-  (*     tr_expression r s' a -> *)
-  (*     tr_stmt (CStan.Sifthenelse r CStan.Sskip CStan.Sskip) (Ssequence s' Sskip) *)
-  (* | tr_ifthenelse: forall r s1 s2 s' a ts1 ts2, *)
-  (*     tr_expression r s' a -> *)
-  (*     tr_stmt s1 ts1 -> tr_stmt s2 ts2 -> *)
-  (*     tr_stmt (CStan.Sifthenelse r s1 s2) (Ssequence s' (Sifthenelse a ts1 ts2)) *)
-  (* | tr_loop: forall r s1 s' ts1, *)
-  (*     tr_if r Sskip Sbreak s' -> *)
-  (*     tr_stmt s1 ts1 -> *)
-  (*     tr_stmt (CStan.Swhile r s1) *)
-  (*             (Sloop (Ssequence s' ts1) Sskip) *)
-  (* | tr_break: *)
-  (*     tr_stmt CStan.Sbreak Sbreak *)
-  (* | tr_continue: *)
-  (*     tr_stmt CStan.Scontinue Scontinue *)
-  (* | tr_return_none: *)
-  (*     tr_stmt (CStan.Sreturn None) (Sreturn None) *)
-  (* | tr_return_some: forall r s' a, *)
-  (*     tr_expression r s' a -> *)
-  (*     tr_stmt (CStan.Sreturn (Some r)) (Ssequence s' (Sreturn (Some a))) *)
-  (* . *)
-
-Inductive tr_function: CStan.function -> Clight.function -> Prop :=
-  | tr_function_intro: forall f tf,
-      tr_stmt f.(CStan.fn_body) tf.(fn_body) ->
-      fn_return tf = CStan.fn_return f ->
-      fn_callconv tf = CStan.fn_callconv f ->
-      (* fn_params tf = CStan.fn_params f -> *)
-      fn_vars tf = CStan.fn_vars f ->
-      tr_function f tf.
-
-
-Inductive tr_fundef: CStan.fundef -> Clight.fundef -> Prop :=
-  | tr_internal: forall f tf,
-      tr_function f tf ->
-      tr_fundef (Internal f) (Internal tf)
-  | tr_external: forall ef targs tres cconv,
-      tr_fundef (External ef targs tres cconv) (External ef targs tres cconv).
-
-Lemma tr_type: CStan.type -> Ctypes.type -> Prop. Admitted.
-
-(** ** Linking types *)
-Lemma cstan_type_eq: forall (ty1 ty2: CStan.type), {ty1=ty2} + {ty1<>ty2}.
-Proof.
-  decide equality.
-  - decide equality.
-  - decide equality. Admitted.
-
+(* --_-_-_-_---                            --_-_-_-_--- *)
+(*     -_-_-     d$$$$"   d$$$$"  d$$$$"       -_-_-    *)
+(*      -__-    **$$$"   **$$$"  **$$$"         -__-    *)
+(*     _-_      .$$$$$"  .$$$$$" .$$$$$"       _-_      *)
+(*    _-           z$"      z$"     z$"       _-        *)
+(*    -_          zP       zP      zP         -_        *)
+(*     _-        ,"       ,"      ,"           _-       *)
+(*                                                      *)
+(*      ░█▀▄░█▀█░█▀█░█▀▀░█▀▀░█▀▄░░░▀▀█░█▀█░█▀█░█▀▀      *)
+(*      ░█░█░█▀█░█░█░█░█░█▀▀░█▀▄░░░▄▀░░█░█░█░█░█▀▀      *)
+(*      ░▀▀░░▀░▀░▀░▀░▀▀▀░▀▀▀░▀░▀░░░▀▀▀░▀▀▀░▀░▀░▀▀▀      *)
+(*                      ,---------,         ,---------, *)
+(*              ,______;       ,____________;           *)
+(*  ,__-----__,-    __'      _;         ,_______,       *)
+(* ;__________;________________________________________ *)
+(* //////////////////////////////////////////////////// *)
 
 Program Instance Linker_types : Linker CStan.type := {
-  link := fun (t1:CStan.type) (t2:CStan.type) => if cstan_type_eq t1 t2 then Some t2 else None;
-  linkorder := fun t1 t2 => t1 = t2
+  link := fun (t1 t2: CStan.type) => None; (* FIXME *)
+  linkorder := fun t1 t2 => t1 = t2; (* FIXME: not a valid preorder *)
 }.
-Next Obligation.
-  destruct (cstan_type_eq x y); inv H. auto.
-Defined.
-
-Global Opaque Linker_types.
 
 Definition match_prog (p: CStan.program) (tp: Clight.program) :=
-  match_program (fun ctx f tf => tr_fundef f tf) (fun t tt => tr_type t tt) p tp
- (* /\ prog_types tp = prog_types p. *)
+  match_program (fun ctx f tf => Sbackend.transf_fundef f = OK tf) (fun cs cl => eq cl (CStan.vd_type cs)) p tp
+  (* /\ prog_types tp = prog_types p. *) (* FIXME: I don't think this is necessary until we get structs. *)
   .
 
+Lemma match_transf_program:
+  forall p tp, Sbackend.backend p = OK tp -> match_prog p tp.
+Proof.
+  unfold Sbackend.backend. intros. monadInv H.
+  eapply match_transform_partial_program2.
+  rewrite EQ. destruct x.
+  Admitted.
+
+Lemma comp_env_preserved:
+  genv_cenv tge = CStan.genv_cenv ge.
+Proof.
+  unfold tge, ge.
+  Admitted.
+(*   destruct tprog. *)
+(*   destruct prog. tprog; simpl. destruct TRANSL as [_ EQ]. simpl in EQ. congruence. *)
+
+(* Qed. *)
+Lemma find_symbol_eq:
+  (* Senv.find_symbol ge = Senv.find_symbol tge -> *)
+  forall i,
+  Genv.find_symbol ge i = Genv.find_symbol tge i.
+Proof.
+  intro.
+  unfold Genv.find_symbol in *.
+  unfold Genv.genv_symb in *.
+  unfold CStan.genv_genv in *.
+  unfold genv_genv in *.
+  simpl in *.
+  Admitted.
+
+
+
+(*      .                       *)
+(*    \ | /      All clear!     *)
+(*  '-.;;;.-'                   *)
+(* -==;;;;;==-                  *)
+(* ---------------------------- *)
+
 Hypothesis TRANSL: match_prog prog tprog.
+
 Lemma senv_preserved:
   Senv.equiv ge tge.
 Proof (Genv.senv_match TRANSL).
+
+Lemma symbols_preserved:
+  forall (s: AST.ident), Genv.find_symbol tge s = Genv.find_symbol ge s.
+Proof (Genv.find_symbol_match TRANSL).
+
+Lemma sizeof_equiv :
+  forall t,
+  sizeof ge t = sizeof tge t.
+Proof.
+  intros.
+  rewrite comp_env_preserved.
+  auto.
+Qed.
+
+Lemma alignof_equiv :
+  forall t,
+  alignof ge t = alignof tge t.
+Proof.
+  rewrite comp_env_preserved.
+  auto.
+Qed.
+
+Lemma transf_types_eq :
+  forall e te,
+  transf_expression e = OK te -> CStan.typeof e = Clight.typeof te.
+Proof.
+  intro e.
+  induction e; intros; inv H;
+    (* base cases *)
+    try (simpl in *; reflexivity);
+
+    (* cases with inductive hypothesis: Ederef, Eunop, Ebinop *)
+    try (monadInv H1;  (* invert our inductive transf_expression *)
+         constructor). (* the rest of the proof follows precisely by constructor *)
+Qed.
 
 Lemma eval_expr_correct:
   forall e le m a v target ta
   (TRE: transf_expression a = OK ta),
   CStan.eval_expr ge e le m target a v -> Clight.eval_expr tge e le m ta v.
 Proof.
-  intros e le m a v target ta.
-  intros.
-  Admitted.
+  intros e le m a.
+  induction a; intros; simpl in TRE; monadInv TRE; simpl.
+
+  (* Econst expressions: *)
+  - (* inversion identifies the eval_Econst_* and eval_lvalue as possibilities *)
+    inv H. (* apply inversion on our CStan.eval_expr *)
+    constructor. (* for eval_Econst_*, apply the corresponding constructor *)
+    inv H0.      (* for eval_lvalue, inversion on the new hypothesis shows that the pattern is invalid *)
+  - inv H. constructor. inv H0.
+  - inv H. constructor. inv H0.
+  - inv H; try constructor; inv H0.
+
+  - (* Evar expressions *)
+    inv H. (* apply inversion on our CStan.eval_expr, this matches eval_lvalue. *)
+    eapply eval_Elvalue.
+    (* redo *)
+
+    Focus 2. (* examine the new deref clauses first *)
+    inv H1; simpl in *.
+    eapply Clight.deref_loc_value; eauto.
+    eapply Clight.deref_loc_reference; eauto.
+    eapply Clight.deref_loc_copy; eauto.
+
+    inv H0.
+    eapply eval_Evar_local. eauto.
+    eapply eval_Evar_global; eauto.
+    rewrite symbols_preserved. eauto.
+
+  - (* Etempvar expressions *)
+    inv H.
+    constructor. exact H3. inv H0.
+
+  (* Inductive-hypotheses *)
+
+  - (* Ederef expressions *)
+    inv H. (* invert with CStan.eval_lvalue... *)
+    inv H0. (* but look! we can only load variables. *)
+
+  - (* Eunop expressions *)
+    inv H.                               (* invert with CStan.eval_Eunop -- we must additionally show CStan.eval_lvalue is invalid. *)
+    econstructor.                        (* apply Clight.eval_Eunop -- we must additionally show Cop.sem_unary_operation *)
+    apply (IHa v1 target x EQ H4).       (* Eunop is then shown to be valid by inductive case of it's argument *)
+    rewrite (transf_types_eq a x) in H5.
+    exact H5. exact EQ.                  (* Cop.sem_unary_operation is true by transf_types_eq, so long as EQ *)
+    inv H0.                              (* CStan.eval_lvalue is invalid. *)
+
+  - (* Ebinop expressions *)
+    inv H.                                 (* invert with CStan.eval_Ebinop *)
+    Focus 2. inv H0.                       (* this also pattern-matches on the invalid CStan.eval_lvalue -- just deal with that now. *)
+    econstructor.                          (* apply Clight.eval_Ebinop *)
+    apply (IHa1 v1 target x EQ H5).        (* The first argument is then proven true by the first inductive case*)
+    apply (IHa2 v2 target x0 EQ1 H6).      (* The second argument is then proven true by the second inductive case*)
+
+    rewrite (transf_types_eq a1 x ) in H7. (* we additionally need to show that Cop.sem_binary_operation is true. *)
+    rewrite (transf_types_eq a2 x0) in H7.
+    rewrite comp_env_preserved.
+    eauto.
+    eauto.
+    eauto.
+
+  (* Two more base cases *)
+
+  - (* Esizeof expressions *)
+    inv H.
+    rewrite sizeof_equiv.
+    apply Clight.eval_Esizeof.
+    inv H0.
+
+  - (* Ealignof expressions *)
+    inv H.
+    rewrite alignof_equiv.
+    apply Clight.eval_Ealignof.
+    inv H0.
+Qed.
 
 Lemma eval_lvalue_correct:
   forall e le m a b ofs target ta
   (TRE: transf_expression a = OK ta),
   CStan.eval_lvalue ge e le m target a b ofs -> Clight.eval_lvalue tge e le m ta b ofs.
 Proof.
-  intros.
-Admitted.
+  intros e le m a.
+  induction a; intros; monadInv TRE; try (inv H).
+  - econstructor. eauto.
+  - eapply eval_Evar_global; eauto.
+    rewrite symbols_preserved. auto.
+Qed.
 
 Lemma types_correct:
   forall e x, transf_expression e = OK x -> CStan.typeof e = Clight.typeof x.
